CertiGC/verif_do_generation.v
@@ -7,100 +7,92 @@ Proof.
   start_function.
   pose proof H. pose proof H0. destruct H2 as [? _]. destruct H3 as [? [? [? _]]].
   assert (generation_space_compatible
-            g (from, nth_gen g from, nth_space (ti_heap t_info) from)) by
+            g (from, nth_gen g from, nth_space h from)) by
       (apply gt_gs_compatible; assumption). destruct H6 as [? [? ?]].
-  assert (generation_space_compatible g (to, nth_gen g to, nth_space (ti_heap t_info) to)) by
+  assert (generation_space_compatible g (to, nth_gen g to, nth_space h to)) by
       (apply gt_gs_compatible; assumption). destruct H9 as [? [? ?]].
-  assert (isptr (space_start (nth_space (ti_heap t_info) from))) by
+  assert (isptr (space_start (nth_space h from))) by
       (rewrite <- H6; apply start_isptr).
-  assert (isptr (space_start (nth_space (ti_heap t_info) to))) by
+  assert (isptr (space_start (nth_space h to))) by
       (rewrite <- H9; apply start_isptr).
   assert (HS: forall gen, graph_has_gen g gen -> Z.of_nat gen < MAX_SPACES). {
     intros. unfold graph_has_gen in H14. destruct H as [[_ [_ ?]] _].
-    rewrite <- (spaces_size (ti_heap t_info)). rewrite Zlength_correct.
+    rewrite <- (spaces_size h). rewrite Zlength_correct.
     apply inj_lt. apply Nat.lt_le_trans with
                       (Datatypes.length (g_gen (glabel g))); assumption. }
   assert (Z.of_nat from < MAX_SPACES) by (apply HS; assumption).
   assert (Z.of_nat to < MAX_SPACES) by (apply HS; assumption). clear HS.
-  freeze [0;1;2] FR.
-  localize [space_struct_rep sh (ti_heap_p t_info) (ti_heap t_info) from; 
-            space_struct_rep sh (ti_heap_p t_info) (ti_heap t_info) to].
+  freeze [0;1;2;3] FR.
+  localize [space_struct_rep sh hp h from; 
+            space_struct_rep sh hp h to].
   unfold space_struct_rep. unfold space_tri.
   forward.
   gather_SEP
     (data_at sh space_type
-             _ (space_address (ti_heap_p t_info) from))
+             _ (space_address hp from))
     (data_at sh space_type
-             _ (space_address (ti_heap_p t_info) to)).
-  replace_SEP 0 (space_struct_rep sh (ti_heap_p t_info) (ti_heap t_info) from 
-                  * space_struct_rep sh (ti_heap_p t_info) (ti_heap t_info) to) by
+             _ (space_address hp to)).
+  replace_SEP 0 (space_struct_rep sh hp h from 
+                  * space_struct_rep sh hp h to) by
     (unfold space_struct_rep; entailer!).
-  unlocalize [thread_info_rep sh t_info ti].
-  1: apply thread_info_rep_ramif_stable;  assumption.
-  assert_PROP (isptr (space_address (ti_heap_p t_info) to)). {
+  unlocalize [heap_rep sh h hp].
+  1: apply heap_rep_ramif_stable;  assumption.
+  assert_PROP (isptr (space_address hp to)). {
     unfold thread_info_rep, heap_rep. unfold heap_struct_rep.
     unfold space_address. Intros.
     entailer!.
   }
   forward_call. clear H16. 
-    localize [space_struct_rep sh (ti_heap_p t_info) (ti_heap t_info) from].
+    localize [space_struct_rep sh hp h from].
     unfold space_struct_rep, space_tri. 
     forward.
     forward.
-    replace_SEP 0 (space_struct_rep sh (ti_heap_p t_info) (ti_heap t_info) from) by
+    replace_SEP 0 (space_struct_rep sh hp h from) by
         (unfold space_struct_rep, space_tri; entailer!).
-    unlocalize [thread_info_rep sh t_info ti].
-    1: apply thread_info_rep_ramif_stable_1; assumption. apply dgc_imply_fc in H0.
-    remember (space_start (nth_space (ti_heap t_info) from)) as from_p.
-    remember (space_start (nth_space (ti_heap t_info) to)) as to_p.
-    remember (WORD_SIZE * used_space (nth_space (ti_heap t_info) to))%Z as to_used.
-    remember (WORD_SIZE * total_space (nth_space (ti_heap t_info) to))%Z as to_total.
-    remember (WORD_SIZE * used_space (nth_space (ti_heap t_info) from))%Z as from_used.
+    unlocalize [heap_rep sh h hp].
+    1: apply heap_rep_ramif_stable_1; assumption. apply dgc_imply_fc in H0.
+    remember (space_start (nth_space h from)) as from_p.
+    remember (space_start (nth_space h to)) as to_p.
+    remember (WORD_SIZE * used_space (nth_space h to))%Z as to_used.
+    remember (WORD_SIZE * total_space (nth_space h to))%Z as to_total.
+    remember (WORD_SIZE * used_space (nth_space h from))%Z as from_used.
     destruct H0 as [? [? ?]]. 
     replace from_p with (gen_start g from) by
         (subst; unfold gen_start; rewrite if_true; assumption).
-    replace (offset_val (WORD_SIZE * total_space (nth_space (ti_heap t_info) from))
-                        (gen_start g from)) with (limit_address g (ti_heap t_info) from) by
+    replace (offset_val (WORD_SIZE * total_space (nth_space h from))
+                        (gen_start g from)) with (limit_address g h from) by
         (unfold limit_address, gen_size; reflexivity).
-    assert_PROP (isptr (space_address (ti_heap_p t_info) to)). {
+    assert_PROP (isptr (space_address hp to)). {
       unfold space_address. rewrite isptr_offset_val. unfold thread_info_rep, heap_rep.
       Intros. unfold heap_struct_rep. entailer!. }
-    assert_PROP (offset_val WORD_SIZE (space_address (ti_heap_p t_info) to) =
-                 next_address t_info to). {
-      unfold thread_info_rep, heap_rep. unfold heap_struct_rep. Intros. entailer!.
-      unfold space_address, next_address, field_address. rewrite if_true.
+    assert_PROP (offset_val WORD_SIZE (space_address hp to) =
+                 heap_next_address hp to). {
+      unfold heap_rep. unfold heap_struct_rep. Intros. entailer!.
+      unfold space_address, heap_next_address, field_address. rewrite if_true.
       - simpl. rewrite offset_offset_val. f_equal.
       - destruct H as [[_ [_ ?]] _]. unfold field_compatible in *.
         simpl in *. unfold in_members. simpl. intuition. } thaw FR.
-    forward_call (rsh, sh, gv, ti, g, t_info, roots, outlier, from, to).
-    1: intuition. Intros vret. destruct vret as [[g1 t_info1] roots1]. simpl fst in *.
-    simpl snd in *. freeze [0;1;2] FR.  
-    replace (space_address (ti_heap_p t_info) from) with (space_address (ti_heap_p t_info1) from) by
-        (unfold space_address; rewrite (proj1 H23); reflexivity).
-    assert (space_start (nth_space (ti_heap t_info1) from) = gen_start g1 from). {
+    forward_call (rsh, sh, gv, g, h, hp, fr, roots, outlier, from, to).
+    1: intuition. Intros vret. destruct vret as [[[g1 h1] fr1] roots1]. simpl fst in *.
+    simpl snd in *. freeze [0;1;2;3] FR.  
+    assert (space_start (nth_space h1 from) = gen_start g1 from). {
       destruct H20 as [? _]. destruct H22 as [_ [? _]]. 
       destruct (gt_gs_compatible _ _ H20 _ H22) as [H24 _]. simpl in H24. rewrite <- H24.
       unfold gen_start. rewrite if_true by assumption. reflexivity. }
-    assert (isptr (space_start (nth_space (ti_heap t_info1) from))). {
+    assert (isptr (space_start (nth_space h1 from))). {
       rewrite H24. unfold gen_start. destruct H22 as [_ [? _]].
       rewrite if_true by assumption. apply start_isptr. }
-    localize [space_struct_rep sh (ti_heap_p t_info1) (ti_heap t_info1) from].
+    localize [space_struct_rep sh hp h1 from].
     unfold space_struct_rep, space_tri. 
     do 2 forward.
-    replace_SEP 0 (space_struct_rep sh (ti_heap_p t_info1) (ti_heap t_info1) from) by
+    replace_SEP 0 (space_struct_rep sh hp h1 from) by
         (unfold space_struct_rep, space_tri; entailer!).
-    unlocalize [thread_info_rep sh t_info1 ti].
-    1: apply thread_info_rep_ramif_stable_1; assumption. thaw FR. rewrite H24.
-    replace (offset_val (WORD_SIZE * total_space (nth_space (ti_heap t_info1) from))
-                        (gen_start g1 from)) with (limit_address g1 (ti_heap t_info1) from) by
+    unlocalize [heap_rep sh h1 hp].
+    1: apply heap_rep_ramif_stable_1; assumption. thaw FR. rewrite H24.
+    replace (offset_val (WORD_SIZE * total_space (nth_space h1 from))
+                        (gen_start g1 from)) with (limit_address g1 h1 from) by
         (unfold limit_address, gen_size; reflexivity).
-    assert_PROP (offset_val WORD_SIZE (space_address (ti_heap_p t_info) to) =
-                 next_address t_info1 to). {
-      unfold thread_info_rep, heap_rep. unfold heap_struct_rep. entailer!.
-      unfold space_address, next_address, field_address. rewrite (proj1 H23), if_true.
-      - simpl. rewrite offset_offset_val. f_equal.
-      - unfold field_compatible in *. simpl.
-        unfold in_members. simpl. intuition. }
+    pose proof I.
     assert (closure_has_v g (to, number_of_vertices (nth_gen g to))) by
         (red; simpl; unfold closure_has_index; split; [assumption | lia]).
     replace (offset_val to_used to_p) with
@@ -111,31 +103,55 @@ Proof.
          rewrite offset_offset_val, H11, H9, if_true by assumption;
          f_equal; unfold WORD_SIZE; lia). eapply frr_closure_has_v in H27; eauto.
     destruct H27. simpl in H27, H28.
-    assert (0 < gen_size (ti_heap t_info1) to) by (rewrite <- (proj1 (proj2 H23)); assumption).
+    assert (0 < gen_size h1 to) by (rewrite <- (proj1 H23); assumption).
     assert (gen_unmarked g1 to) by (eapply (frr_gen_unmarked _ _ _ g _ g1); eauto).
-    forward_call (rsh, sh, gv, ti, g1, t_info1, roots1, outlier,
+    sep_apply frames_rep_localize. Intros.
+    forward_call (rsh, sh, gv, g1, h1, hp, frames2rootpairs fr1, roots1, outlier,
                   from, to, number_of_vertices (nth_gen g to)).
-    Intros vret. destruct vret as [g2 t_info2]. simpl fst in *. simpl snd in *.
-    replace (space_address (ti_heap_p t_info1) from) with (space_address (ti_heap_p t_info2) from) in * by
-        (unfold space_address; rewrite (proj1 H34); reflexivity).
-    assert (space_start (nth_space (ti_heap t_info2) from) = gen_start g2 from). {
+    Intros vret.
+    destruct vret as [[g2 h2] rootpairs2]. simpl fst in *. simpl snd in *.
+    assert (ADRS: map rp_adr rootpairs2 = map rp_adr (frames2rootpairs fr1)). {
+      clear H34 H33 H32 MORE_COMMANDS H30 H29 H28 H27 H26 H25 H24.
+      clear H21 H22 H23.
+      red in H20, H31.
+      destruct H20 as [_ [H20b [[H20c H20d] _]]].
+      destruct H31 as [_ [H31b [[H31c H31d] _]]].
+      red in H20b,H20c,H20d,H31b,H31c, H31d.
+      Print rootpairs_compatible.
+      admit.
+    }
+    sep_apply frames_rep_unlocalize.
+    set (fr2 := update_frames fr1 (map rp_val rootpairs2)).
+    (*
+    gather_SEP 0 4 5.
+    replace_SEP 0 (thread_info_rep sh t_info2 ti). {
+      subst t_info2. unfold thread_info_rep.
+      entailer!. simpl. cancel.
+      apply derives_refl'; f_equal. f_equal. f_equal. f_equal.
+      f_equal. f_equal. unfold ti_fp.
+      simpl. rewrite frames_p_update_frames. auto.
+    }
+    *)
+    assert (space_start (nth_space h2 from) = gen_start g2 from). {
       destruct H31 as [? _]. destruct H32 as [_ [? _]].
-      destruct (gt_gs_compatible _ _ H31 _ H32) as [? _]. simpl in H35. rewrite <- H35.
+      destruct (gt_gs_compatible _ _ H31 _ H32) as [? _]. simpl in H35.
+      rewrite <- H35.
       unfold gen_start. rewrite if_true by assumption. reflexivity. }
-    assert (isptr (space_start (nth_space (ti_heap t_info2) from))). {
+    assert (isptr (space_start (nth_space h2 from))). {
       rewrite H35. unfold gen_start. destruct H32 as [_ [? _]].
       rewrite if_true by assumption. apply start_isptr. } 
-    freeze [0;1;2] FR. localize [space_struct_rep sh (ti_heap_p t_info2) (ti_heap t_info2) from].
+    freeze [0;1;2;3] FR. localize [space_struct_rep sh hp h2 from].
     unfold space_struct_rep, space_tri.
     forward.
-    replace_SEP 0 (space_struct_rep sh (ti_heap_p t_info2) (ti_heap t_info2) from) by
+    replace_SEP 0 (space_struct_rep sh hp h2 from) by
         (unfold space_struct_rep, space_tri; entailer!).
-    unlocalize [thread_info_rep sh t_info2 ti].
-    1: apply thread_info_rep_ramif_stable_1; assumption. thaw FR.
-    unfold thread_info_rep, heap_rep. Intros. freeze [0;1;3;4;6] FR. rewrite heap_struct_rep_eq.
-    assert_PROP (space_address (ti_heap_p t_info2) from =
+    unlocalize [heap_rep sh h2 hp].
+    1: apply heap_rep_ramif_stable_1; assumption. thaw FR.
+    unfold thread_info_rep, heap_rep. Intros.
+    freeze [1;2;3;5] FR. rewrite heap_struct_rep_eq.
+    assert_PROP (space_address hp from =
                  field_address (tarray space_type MAX_SPACES) [ArraySubsc (Z.of_nat from)]
-                               (ti_heap_p t_info2)). {
+                               hp). {
       entailer!. unfold space_address. unfold field_address. rewrite if_true.
       - simpl. f_equal.
       - unfold field_compatible in *. simpl in *. intuition. }
@@ -143,7 +159,7 @@ Proof.
     rewrite Znth_map by (rewrite spaces_size; rep_lia).
     rewrite <- nth_space_Znth. unfold space_tri at 2 3.
     simpl fst. simpl snd.
-    assert (FROM_MAX: 0 <= Z.of_nat from < Zlength (map space_tri (spaces (ti_heap t_info2)))). {
+    assert (FROM_MAX: 0 <= Z.of_nat from < Zlength (map space_tri (spaces h2))). {
         rewrite Zlength_map.
         destruct H20 as [[_ [_ ?]] _]; destruct H31 as [[_ [_ H31]] _]. simpl in H31.
         apply frr_graph_has_gen with (gen:=from) in H21; auto.
@@ -163,14 +179,15 @@ Proof.
     thaw FR.
     assert (graph_has_gen g2 from) by (destruct H32 as [_ [? _]]; assumption).
     rewrite (graph_rep_reset g2 from) by assumption. Intros.     
-    sep_apply (heap_rest_rep_reset g2 (ti_heap t_info2) from (proj1 H31) H37).
+    sep_apply (heap_rest_rep_reset g2 h2 from (proj1 H31) H37).
         rewrite <- heap_struct_rep_eq.
-    gather_SEP (data_at _ _ _ _) (frames_rep _ _) (heap_struct_rep _ _ _) (heap_rest_rep _).
-    replace_SEP 0 (thread_info_rep sh (reset_nth_heap_thread_info from t_info2) ti).
-    + unfold thread_info_rep, heap_rep. simpl ti_heap_p. simpl ti_args. entailer!.
-      assert (from < length (spaces (ti_heap t_info2)))%nat by
+    simpl fst. simpl snd.
+    gather_SEP 0 4. 
+    replace_SEP 0 (heap_rep sh (reset_nth_heap from h2) hp).
+    + unfold heap_rep. entailer!.
+      assert (from < length (spaces h2))%nat by
           (destruct H31 as [[_ [_ ?]] _]; simpl in H31; red in H37; lia). simpl.
-      rewrite (reset_nth_space_Znth _ _ H49), <- nth_space_Znth, <- upd_Znth_map.
+      rewrite (reset_nth_space_Znth _ _ H48), <- nth_space_Znth, <- upd_Znth_map.
       unfold space_tri at 3. simpl. replace (WORD_SIZE * 0)%Z with 0 by lia.
       rewrite isptr_offset_val_zero by assumption. cancel.
     + apply super_compatible_reset with (gen := from) in H31.
@@ -179,15 +196,25 @@ Proof.
            - clear -H. destruct H as [_ [_ [[_ ?] _]]]. assumption.
            - apply frl_roots_Zlength in H21; auto. 
       }
-      remember (reset_nth_heap_thread_info from t_info2) as t_info3.
+      remember (reset_nth_heap from h2) as h3.
       remember (reset_graph from g2) as g3.
       assert (do_generation_relation from to roots roots1 g g3) by
           (exists g1, g2; split; [|split]; assumption).
-      assert (thread_info_relation t_info t_info3). {
-        apply tir_trans with t_info2.
-        - apply tir_trans with t_info1; assumption.
-        - subst t_info3. apply tir_reset. }      
-      Exists g3 t_info3 roots1.
-      destruct H32 as [? [? [? ?]]]. entailer!.
+      assert (heap_relation h h3). {
+        apply hr_trans with h2.
+        - apply hr_trans with h1; try assumption.
+        - subst h3. apply heaprel_reset. }      
+      Exists g3 h3 fr2 roots1.
+      destruct H32 as [? [? [? ?]]].
+      assert (frames2rootpairs fr2 = rootpairs2). {
+          subst fr2.
+          rewrite <- update_rootpairs_frames2rootpairs.
+          clear - ADRS.
+          Search update_rootpairs.
+          admit.
+          admit.
+      }
+      rewrite H43 in *.
+      entailer!.
 Qed.
 
